Consolidate the integer helpers
This isn't really a library since the rest of the code directly uses
Word functions/theorems on u64, but it has some helpers and plugs into
the stdpp ecosystem.

src/Helpers/Integers.v
@@ -8,8 +8,30 @@ Open Scope N_scope.
 (* this is sort of a big number *)
 Definition n64: nat := 64.
 Notation u64 := (word n64).
-Definition u64_max : N := Npow2 n64.
-Opaque u64_max.
+
+(* TODO: to make minimal changes to heap_lang we use Z as the "model" for
+integers in several places; these should be replaced by u64 itself where
+possible and N elsewhere. *)
+Definition u64_Z (x:u64) : Z :=
+  Z.of_N (Word.wordToN x).
+
+Set Printing Coercions.
+
+Theorem u64_Z_through_nat : forall (x:u64), Z.of_nat (Word.wordToNat x) = u64_Z x.
+Proof.
+  unfold u64_Z; intros.
+  rewrite Word.wordToN_nat.
+  rewrite nat_N_Z; auto.
+Qed.
+
+Theorem u64_nat_through_Z : forall (x:u64), Z.to_nat (u64_Z x) = Word.wordToNat x.
+Proof.
+  unfold u64_Z; intros.
+  rewrite N_Z_nat_conversions.N_to_Z_to_nat.
+  rewrite Word.wordToN_to_nat; auto.
+Qed.
+
+Unset Printing Coercions.
 
 Instance word_eq_dec sz : EqDecision (word sz) := @weq sz.
 Instance word_countable sz : Countable (word sz).
@@ -22,20 +44,7 @@ Qed.
 
 Instance wlt_decide sz : Decision (@wlt sz x y) := @wlt_dec sz.
 
-(* TODO: note that these wrappers are inconvenient so we're actually using word
-functions directly; if the indirection is useful we can add it and make u64
-opaque *)
-
-Definition add_u64 : u64 -> u64 -> u64 := @wplus _.
-Definition minus_u64 : u64 -> u64 -> u64 := @wminus _.
-Definition mult_u64 : u64 -> u64 -> u64 := @wmult _.
-
-Definition u64_v : u64 -> N := @wordToN _.
-
-Theorem u64_bound : forall (x:u64), u64_v x < u64_max.
-Proof.
-  intros.
-  apply wordToN_bound.
-Qed.
-
 Definition byte := (word 8).
+
+(* we don't actually do anything with a byte except use its zero value and
+encode integers into bytes, so nothing operates on bytes for now. *)
